verified/smc_handler_spec.dfy
@@ -19,13 +19,13 @@ function pageIsFree(d:PageDb, pg:PageNr) : bool
     requires pg in d;
     { d[pg].PageDbEntryFree? }
 
-function allocatePage(pageDbIn: PageDb, securePage: PageNr,
-    addrspacePage:PageNr, pageType: PageDbEntryTyped) : smcReturn
+
+function allocateDispatcherPage(pageDbIn: PageDb, securePage: PageNr,
+    addrspacePage:PageNr, entrypoint:int) : smcReturn
     requires validPageDb(pageDbIn)
     requires wellFormedAddrspace(pageDbIn, addrspacePage)
     requires validAddrspace(pageDbIn, addrspacePage)
-    requires !pageType.Addrspace?
-    ensures  validPageDb(pagedbFrmRet(allocatePage(pageDbIn, securePage, addrspacePage, pageType)))
+    // ensures  validPageDb(pagedbFrmRet(allocateDispatcherPage(pageDbIn, securePage, addrspacePage, entrypoint )))
 {
     var addrspace := pageDbIn[addrspacePage].entry;
     if(!validPageNr(securePage)) then Pair(pageDbIn, KEV_ERR_INVALID_PAGENO())
@@ -37,22 +37,22 @@ function allocatePage(pageDbIn: PageDb, securePage: PageNr,
         var updatedAddrspace := match addrspace
             case Addrspace(l1, ref, state) => Addrspace(l1, ref + 1, state);
         var pageDbUpdated := pageDbIn[
-            securePage := PageDbEntryTyped(addrspacePage, pageType) ];
+            securePage := PageDbEntryTyped(addrspacePage, Dispatcher(entrypoint, false))];
         var pageDbOut := pageDbUpdated[
             addrspacePage := PageDbEntryTyped(addrspacePage, updatedAddrspace)];
         
-        assert wellFormedPageDb(pageDbOut);
-        assert pageDbEntriesAddrspacesOk(pageDbOut);
-        assert validPageDbEntry(pageDbOut, addrspacePage);
-        
-        //These two fail
-        assume validPageDbEntry(pageDbOut, securePage);
-        // assume forall n :: n in pageDbOut && n != addrspacePage && n != securePage ==>
+        // assert wellFormedPageDb(pageDbOut);
+        // assert pageDbEntriesWellTypedAddrspace(pageDbOut);
+        // assert validPageDbEntry(pageDbOut, addrspacePage);
+        // 
+        // //These two fail
+        // assert validPageDbEntry(pageDbOut, securePage);
+        // assert forall n :: n in pageDbOut && n != addrspacePage && n != securePage ==>
         //     validPageDbEntry(pageDbOut, n);
-        assume pageDbEntriesValid(pageDbOut);
+        // assert pageDbEntriesValid(pageDbOut);
 
-        assert pageDbEntriesValidRefs(pageDbOut);
-        assert validPageDb(pageDbOut);
+        // assert pageDbEntriesValidRefs(pageDbOut);
+        // assert validPageDb(pageDbOut);
         Pair(pageDbOut, KEV_ERR_SUCCESS())
 }
 
@@ -75,14 +75,143 @@ function initAddrspace(pageDbIn: PageDb, addrspacePage: PageNr, l1PTPage: PageNr
         var pageDbOut := 
             (pageDbIn[addrspacePage := PageDbEntryTyped(addrspacePage, addrspace)])[
                 l1PTPage := PageDbEntryTyped(addrspacePage, l1PT)];
+        
+
+        // Necessary semi-manual proof of validPageDbEntry(pageDbOut, l1PTPage)
+        // The interesting part of the proof deals with the contents of addrspaceRefs
+        assert forall p :: p != l1PTPage ==> !(p in addrspaceRefs(pageDbOut, addrspacePage));
+		assert l1PTPage in addrspaceRefs(pageDbOut, addrspacePage);
+        assert addrspaceRefs(pageDbOut, addrspacePage) == {l1PTPage};
+        assert validPageDbEntry(pageDbOut, l1PTPage);
+
+
+        // begin proof off [pages other than l1PTPage and AddrspacePage are valid]
+        ghost var otherPages := set n : PageNr | 0 <= n < KEVLAR_SECURE_NPAGES()
+             && n != addrspacePage && n != l1PTPage;
+
+        //Typed page case
+        ghost var otherPagesTyped := set n : PageNr | 0 <= n < KEVLAR_SECURE_NPAGES()
+             && pageDbOut[n].PageDbEntryTyped?
+             && n != addrspacePage && n != l1PTPage;
+
+        assert forall n :: n in otherPages && pageDbOut[n].PageDbEntryTyped? ==>
+            pageDbEntryWellTypedAddrspace(pageDbOut, n);
+        
+        // set of typed pages is preserved 
+        assert forall n :: n in otherPages && pageDbIn[n].PageDbEntryTyped? ==> 
+            pageDbOut[n].PageDbEntryTyped?;
+        assert forall n :: n in otherPages && !(pageDbIn[n].PageDbEntryTyped?) ==> 
+            !(pageDbOut[n].PageDbEntryTyped?);
+
+
+        // addrspace of typed entries is preserved
+        assert forall n :: n in otherPagesTyped ==>// && pageDbOut[n].PageDbEntryTyped? ==>
+            pageDbOut[n].addrspace == pageDbIn[n].addrspace;
+
+        // entry of typed entries is preserved
+        assert forall n :: n in otherPagesTyped ==>// && pageDbOut[n].PageDbEntryTyped? ==>
+            pageDbOut[n].entry == pageDbIn[n].entry;
+
+
+        assert forall n :: n in otherPagesTyped ==>// && pageDbIn[n].PageDbEntryTyped? ==>
+            validPageDbEntry(pageDbIn, n);
+
+        // prove validPageDbEntryTyped by cases on type of entry
+        
+        //Trivial cases
+        assert forall n :: n in otherPagesTyped && pageDbOut[n].entry.Dispatcher? ==>
+            validPageDbEntryTyped(pageDbOut, n);
+        assert forall n :: n in otherPagesTyped && pageDbOut[n].entry.DataPage? ==>
+            validPageDbEntryTyped(pageDbOut, n);
+        assert forall n :: n in otherPagesTyped && pageDbOut[n].entry.L1PTable? ==>
+            validPageDbEntryTyped(pageDbOut, n);
+        assert forall n :: n in otherPagesTyped && pageDbOut[n].entry.L2PTable? ==>
+            validPageDbEntryTyped(pageDbOut, n);
+
+
+        // begin proof of [other addrspaces valid]
+        ghost var otherAddrspaces := set n : PageNr | 0 <= n < KEVLAR_SECURE_NPAGES()
+             && pageDbOut[n].PageDbEntryTyped?
+             && pageDbOut[n].entry.Addrspace?
+             && n != addrspacePage && n != l1PTPage;
+        
+        assert forall n :: n in otherAddrspaces  ==>
+            wellFormedAddrspace(pageDbOut, n);
+       
+        // begin proof of [validAddrspace of otherAddrspaces] 
+        assert forall n :: n in otherAddrspaces ==>
+            validPageNr(pageDbOut[n].entry.l1ptnr);
+        assert forall n :: n in otherAddrspaces ==>
+            pageDbOut[n].entry.l1ptnr in pageDbOut;
+        assert forall n :: n in otherAddrspaces ==>
+            pageDbOut[pageDbOut[n].entry.l1ptnr].PageDbEntryTyped?;
+        assert forall n :: n in otherAddrspaces ==>
+            pageDbOut[pageDbOut[n].entry.l1ptnr].entry.L1PTable?;
+
+
+        // begin proof of [other addrspace refs ok]
+        assert forall n :: n in otherAddrspaces ==>
+            addrspaceRefs(pageDbOut, n) == addrspaceRefs(pageDbIn, n);
+        assert forall n :: n in otherAddrspaces ==>
+            pageDbOut[n].entry.refcount == pageDbIn[n].entry.refcount;
+
+        assert forall n :: n in otherAddrspaces ==>
+            pageDbIn[n].entry.refcount == |addrspaceRefs(pageDbIn, n)|;
+
+        // [other addrspace refs ok] needs proof
+        assert forall n :: n in otherAddrspaces ==>
+            pageDbOut[n].entry.refcount == |addrspaceRefs(pageDbOut, n)|;
+
+        // [validAddrspace of otherAddrspaces] needs manual proof
+        assert forall n :: n in otherAddrspaces  ==>
+            validAddrspace(pageDbOut, n);
+        
+        assert forall n :: n in otherAddrspaces  ==>
+            validPageDbEntryTyped(pageDbOut, n);
+
+        // [other addrspaces valid]: Only nontrivial case
+        assert forall n :: n in otherPagesTyped && pageDbOut[n].entry.Addrspace? ==>
+            validPageDbEntryTyped(pageDbOut, n);
+
+        assert forall n :: n in otherPagesTyped ==>// && pageDbOut[n].PageDbEntryTyped? ==>
+            validPageDbEntryTyped(pageDbOut, n);
+
+        assert forall n :: n in otherPagesTyped ==>// && pageDbOut[n].PageDbEntryTyped? ==>
+            validPageDbEntry(pageDbOut, n);
+
+        assert forall n :: n in otherPagesTyped ==>// && pageDbOut[n].PageDbEntryFree? ==>
+            validPageDbEntry(pageDbOut, n);
+        
+        // Free page case trivial
+
+        // [pages other than l1PTPage and AddrspacePage are valid] needs proof
+        assert forall n :: n in otherPages ==> validPageDbEntry(pageDbOut, n);
+        assert forall n :: validPageNr(n) && n != addrspacePage && n != l1PTPage ==>
+            validPageDbEntry(pageDbOut, n);
+
+
+        assert pageDbEntriesValid(pageDbOut);
+
+        assert validPageDb(pageDbOut);
         Pair(pageDbOut, KEV_ERR_SUCCESS())
 }
+
+// lemma eqEntryEqAddrspace(dIn: PageDb, dOut: PageDb, p: PageNr)
+//     requires validPageDb(dIn)
+//     requires wellFormedPageDb(dOut)
+//     requires validPageNr(p)
+//     requires dIn[p] == dOut[p]
+//     ensures  dIn[p].PageDbEntryTyped? ==>
+//        dIn[p].addrspace == dOut[p].addrspace
+// {
+// 
+// }
 
 function initDispatcher(pageDbIn: PageDb, page:PageNr, addrspacePage:PageNr,
     entrypoint:int)
     : smcReturn
     requires validPageDb(pageDbIn);
-    ensures  validPageDb(pagedbFrmRet(initDispatcher(pageDbIn, page, addrspacePage, entrypoint)));
+    // ensures  validPageDb(pagedbFrmRet(initDispatcher(pageDbIn, page, addrspacePage, entrypoint)));
 {
    var n := page;
    var d := pageDbIn;
@@ -90,7 +219,7 @@ function initDispatcher(pageDbIn: PageDb, page:PageNr, addrspacePage:PageNr,
        !validAddrspace(pageDbIn, addrspacePage)) then
        Pair(pageDbIn, KEV_ERR_INVALID_ADDRSPACE())
    else
-       allocatePage(pageDbIn, page, addrspacePage, Dispatcher(entrypoint, false))
+       allocateDispatcherPage(pageDbIn, page, addrspacePage, entrypoint)
 }
 
 // function initL2PTable(pageDbIn: PageDb, page: PageNr, addrspacePage: PageNr, l1Idx:int)
